\documentclass{article}
\usepackage{amsmath}
\usepackage{amssymb}

\begin{document}

\[
\boldsymbol{r}(t) =
\left[
\boldsymbol{u}_d(t) - c_{\text{SFA}} \sum_n \boldsymbol{a}_k(t)
\right]_+
\]

\[
0 < c_{\text{SFA}}
\]

\[
\frac{d \boldsymbol{a}_k}{dt}
= \frac{-\boldsymbol{a}_k + \boldsymbol{r}}{\tau_{a_k}}
\]

\[
\boldsymbol{p} = \boldsymbol{r} \prod_m \boldsymbol{b}_m
\]

\[
\frac{d \boldsymbol{b}_m}{dt}
= \frac{1 - \boldsymbol{b}_m}{\tau_{b_m}} - \frac{F_{\text{STD}}}{\tau_{\text{STD}}} \boldsymbol{p}
\]

\[
0 \leq \boldsymbol{b}_m \leq 1 \qquad F_{\text{STD}} \in \{0, 1\}
\]

\[
\frac{d \boldsymbol{u}_d}{dt}
= \frac{-\boldsymbol{u}_d + \boldsymbol{u}_{\text{ex}} + M * \boldsymbol{p}}{\tau_d}
\]

\end{document} 